Mica/Verifier.lean
@@ -12,7 +12,6 @@ import Mica.Verifier.Intrinsic
 import Mica.Verifier.BoundedQuantifier
 import Mica.Verifier.Expressions
 import Mica.Verifier.RelationalEncoding
-import Mica.Verifier.Functions
 import Mica.Verifier.Specifications
 import Mica.Verifier.SpecMaps
 import Mica.Verifier.Programs
